AczelSetTheory/Axioms/Pair.lean
@@ -4,7 +4,10 @@ import AczelSetTheory.HFSets
 namespace HFSet
 
 /-- Axioma de Pares: x ∈ pair a b ↔ x = a ∨ x = b. -/
-theorem mem_pair (x a b : HFSet) : x ∈ pair a b ↔ x = a ∨ x = b := by
+theorem mem_pair
+  (x a b : HFSet) :
+    x ∈ pair a b ↔ x = a ∨ x = b
+      := by
   rcases Quotient.exists_rep x with ⟨xc, rfl⟩
   rcases Quotient.exists_rep a with ⟨ac, rfl⟩
   rcases Quotient.exists_rep b with ⟨bc, rfl⟩
