AczelSetTheory/Axioms/Powerset.lean
@@ -4,8 +4,10 @@ import AczelSetTheory.Axioms.Separation
 namespace HFSet
 
 /-- Axiona de Conjunto Potencia (Powerset) abstracto. -/
-theorem mem_powerset (A : HFSet) (B : HFSet) :
-    B ∈ powerset A ↔ (∀ x, x ∈ B → x ∈ A) := by
+theorem mem_powerset
+  (A : HFSet) (B : HFSet) :
+    B ∈ powerset A ↔ (∀ x, x ∈ B → x ∈ A)
+      := by
   sorry
 
 end HFSet
